Fixed compiling error I introduced in the previous commit. Also removed redundant sections from cps_util

theories/L6_PCPS/cps_util.v
@@ -8,8 +8,6 @@ Require Import cps.
 (* 
  SUBTERM - proper subterm relation
 
- CTX     - applicative contexts 
-
  OCCUR   - number of occurence of variables
 
  BINDING - list of variable bindings, unique binding property
@@ -28,249 +26,239 @@ Ltac destructAll :=
 
 Definition var_dec := M.elt_eq.
 
-Section SUBTERM.
+Inductive subterm_e: exp -> exp -> Prop :=
+(* immediate *)
+| subterm_constr: forall x t c ys e, subterm_e e (Econstr x t c ys e)
+| subterm_proj: forall v t n y e, subterm_e e (Eproj v t n y e)
+| subterm_prim: forall x t f ys e, subterm_e e (Eprim x t f ys e)
+(* remote *)
+| subterm_constr':
+    forall x t c ys e e', subterm_e e' e -> subterm_e e' (Econstr x t c ys e)
+| subterm_proj':
+    forall v t n y e e', subterm_e e' e -> subterm_e e' (Eproj v t n y e)
+| subterm_prim':
+    forall x t f ys e e', subterm_e e' e -> subterm_e e' (Eprim x t f ys e)
+(* in fdefs *)
+| subterm_fds:
+    forall e' fds e,
+      subterm_fds_e e' fds -> subterm_e e' (Efun fds e)
+with subterm_fds_e: exp -> fundefs -> Prop :=
+     | subterm_cons:
+         forall e f t ys fds', subterm_fds_e e (Fcons f t ys e fds')
+     | subterm_cons':
+         forall e' e f t ys fds', subterm_e e' e -> subterm_fds_e e' (Fcons f t ys e fds')
+     | subterm_cons_fds:
+         forall e' fds' f t ys e , subterm_fds_e e' fds' -> subterm_fds_e e' (Fcons f t ys e fds').
 
-  Inductive subterm_e: exp -> exp -> Prop :=
-  (* immediate *)
-  | subterm_constr: forall x t c ys e,  subterm_e e (Econstr x t c ys e)
-  | subterm_proj: forall v t n y e, subterm_e e (Eproj v t n y e)
-  | subterm_prim: forall x t f ys e, subterm_e e (Eprim x t f ys e)
-  (* remote *)
-  | subterm_constr':
-      forall x t c ys e e', subterm_e e' e -> subterm_e e' (Econstr x t c ys e)
-  | subterm_proj':
-      forall v t n y e e', subterm_e e' e -> subterm_e e' (Eproj v t n y e)
-  | subterm_prim':
-      forall x t f ys e e', subterm_e e' e -> subterm_e e' (Eprim x t f ys e)
-  (* in fdefs *)
-  | subterm_fds:
-      forall e' fds e,
-        subterm_fds_e e' fds -> subterm_e e' (Efun fds e)
-  with subterm_fds_e: exp -> fundefs -> Prop :=
-       | subterm_cons:
-           forall e f t ys fds', subterm_fds_e e (Fcons f t ys e fds')
-       | subterm_cons':
-           forall e' e f t ys fds', subterm_e e' e -> subterm_fds_e e' (Fcons f t ys e fds')
-       | subterm_cons_fds:
-           forall e' fds' f t ys e , subterm_fds_e e' fds' -> subterm_fds_e e' (Fcons f t ys e fds').
-
-  Inductive subfds_fds: fundefs -> fundefs -> Prop :=
-  | subfds_cons':
-      forall fds' fds f t ys e,
-        subfds_fds fds' fds ->
-        subfds_fds fds' (Fcons f t ys e fds)
-  | subfds_cons:
-      forall fds f t ys e, subfds_fds fds (Fcons f t ys e fds).
+Inductive subfds_fds: fundefs -> fundefs -> Prop :=
+| subfds_cons':
+    forall fds' fds f t ys e,
+      subfds_fds fds' fds ->
+      subfds_fds fds' (Fcons f t ys e fds)
+| subfds_cons:
+    forall fds f t ys e, subfds_fds fds (Fcons f t ys e fds).
 
 
-  Definition subterm_or_eq: exp -> exp -> Prop :=
-    fun e' e => subterm_e e' e \/ e' = e.
+Definition subterm_or_eq: exp -> exp -> Prop :=
+  fun e' e => subterm_e e' e \/ e' = e.
 
-  Definition subfds_or_eq: fundefs -> fundefs -> Prop :=
-    fun fds' fds => subfds_fds fds' fds \/ fds' = fds.
+Definition subfds_or_eq: fundefs -> fundefs -> Prop :=
+  fun fds' fds => subfds_fds fds' fds \/ fds' = fds.
 
-  Definition subfds_e: fundefs -> exp -> Prop := 
-    fun fds  e =>
-      exists fds' e', subterm_or_eq (Efun fds' e') e /\  subfds_or_eq fds fds'.
+Definition subfds_e: fundefs -> exp -> Prop := 
+  fun fds  e =>
+    exists fds' e', subterm_or_eq (Efun fds' e') e /\  subfds_or_eq fds fds'.
 
-  Definition subfds_or_eq_left:
-    forall fds' fds fds'',
-      subfds_fds fds fds' -> subfds_or_eq fds' fds'' -> subfds_or_eq fds fds''.
-  Proof.
-    induction fds'; intros.
-    - inversion H; subst. eapply IHfds'. apply H3. admit. admit.
-  Admitted.  
+Definition subfds_or_eq_left:
+  forall fds' fds fds'',
+    subfds_fds fds fds' -> subfds_or_eq fds' fds'' -> subfds_or_eq fds fds''.
+Proof.
+  induction fds'; intros.
+  - inversion H; subst. eapply IHfds'. apply H3. admit. admit.
+Admitted.  
 
-  Theorem subfds_e_subfds:
-    forall fds e fds', subfds_fds fds' fds -> subfds_e fds e -> subfds_e fds' e.
-  Proof.
-    destruct fds; intros.
-    - destruct H0; destructAll. exists x. exists x0. split.
-      assumption.  eapply subfds_or_eq_left. apply H. assumption.
-    - inversion H. 
-  Qed.
-
-End SUBTERM.
-
-Section OCCUR.
-
-  Definition num_occur_list (lv:list var) (v:var) : nat :=
-    fold_right (fun v' n => if (var_dec v v') then 1 + n
-                            else n) 0 lv.
-  
-  (* number of time var occurs in exp (free or not) *)
-  (* Inductive num_occur: exp -> var -> nat -> Prop := *)
-  (* | Num_occ_constr: *)
-  (*   forall x t c ys e v n, *)
-  (*     num_occur e v n -> *)
-  (*     num_occur (Econstr x t c ys e) v (n + (num_occur_list ys v)) *)
-  (* | Num_occ_prim: *)
-  (*     forall x t f ys e v n, *)
-  (*       num_occur e v n -> *)
-  (*       num_occur (Eprim x t f ys e) v (n + (num_occur_list ys v)) *)
-  (* | Num_occ_case: *)
-  (*     forall v' cl v, *)
-  (*       num_occur (Ecase v' cl) v (num_occur_list (v'::(snd (split cl))) v) *)
-  (* | Num_occ_proj: *)
-  (*     forall e v n  y v' t n', *)
-  (*       num_occur  e v n ->  *)
-  (*       num_occur (Eproj v' t n' y e) v (num_occur_list [y] v + n) *)
-  (* | Num_occ_app: *)
-  (*     forall f ys v, *)
-  (*                  num_occur (Eapp f ys) v (num_occur_list (f::ys) v) *)
-  (* | Num_occ_fun: *)
-  (*     forall e v n m fl, *)
-  (*       num_occur e v n -> *)
-  (*       num_occur_fds fl v m -> *)
-  (*       num_occur (Efun fl e) v (n + m ) *)
-  (* with num_occur_fds: fundefs -> var -> nat -> Prop := *)
-  (*      | Num_occ_nil : *)
-  (*          forall v, *)
-  (*            num_occur_fds Fnil v 0 *)
-  (*      | Num_occ_cons : *)
-  (*          forall v t n v' ys e fds' m, *)
-  (*            num_occur e v n -> *)
-  (*            num_occur_fds fds' v m -> *)
-  (*            num_occur_fds (Fcons v' t ys e fds') v (n + m). *)
+Theorem subfds_e_subfds:
+  forall fds e fds', subfds_fds fds' fds -> subfds_e fds e -> subfds_e fds' e.
+Proof.
+  destruct fds; intros.
+  - destruct H0; destructAll. exists x. exists x0. split.
+    assumption.  eapply subfds_or_eq_left. apply H. assumption.
+  - inversion H. 
+Qed.
 
 
-  (* (* number of times var occurs in a context *) *)
-  (* Inductive num_occur_ec: exp_ctx -> var -> nat -> Prop := *)
-  (* | Noec_hole: forall v, num_occur_ec Hole_c v 0 *)
-  (* | Noec_constr: forall c v n x t ys g, *)
-  (*                  num_occur_ec c v n ->  *)
-  (*                  num_occur_ec (Econstr_c x t g ys c) v (num_occur_list ys v + n) *)
-  (* | Noec_prim: forall c v n x t f ys,  *)
-  (*                num_occur_ec c v n ->  *)
-  (*                num_occur_ec (Eprim_c x t f ys c) v (num_occur_list ys v + n ) *)
-  (* | Noec_proj: forall  v n y v' t n' c, *)
-  (*                num_occur_ec c v n -> *)
-  (*                num_occur_ec (Eproj_c v' t n' y c) v (num_occur_list [y] v + n) *)
-  (* | Noec_fun1: forall n m fds c v, *)
-  (*                num_occur_ec c v n -> *)
-  (*                num_occur_fds fds v m -> *)
-  (*                num_occur_ec (Efun1_c fds c) v (n+m) *)
-  (* | Noec_fun2: forall n m fdc e v , *)
-  (*                num_occur e v n -> *)
-  (*                num_occur_fdc fdc v m -> *)
-  (*                num_occur_ec (Efun2_c fdc e) v (n + m) *)
-  (* with num_occur_fdc : fundefs_ctx -> var -> nat -> Prop := *)
-  (*      | Nofc_fcons1 : forall v n m fds t ys c f, *)
-  (*                        num_occur_ec c v n -> *)
-  (*                        num_occur_fds fds v m ->  *)
-  (*                        num_occur_fdc (Fcons1_c f t ys c fds) v  (n + m) *)
-  (*      | Nofc_fcons2 : forall e v n m fdc f t ys, *)
-  (*                        num_occur e v n -> *)
-  (*                        num_occur_fdc fdc v m -> *)
-  (*                        num_occur_fdc (Fcons2_c f t ys e fdc) v (n + m). *)
-  
-  
-  (* (* number of times var occurs in exp in an applied position *) *)
-  (* Inductive num_occur_app: exp -> var -> nat -> Prop := *)
-  (* | Num_oa_constr: *)
-  (*   forall x t c ys e v n, *)
-  (*     num_occur_app e v n -> num_occur_app (Econstr x t c ys e) v n *)
-  (* | Num_oa_prim: *)
-  (*     forall x t f ys e v n, *)
-  (*       num_occur_app e v n -> num_occur_app (Eprim x t f ys e) v n *)
-  (* | Num_oa_case: *)
-  (*     forall v' cl v, *)
-  (*       num_occur_app (Ecase v' cl) v (num_occur_list [v'] v) *)
-  (* | Num_oa_proj: *)
-  (*     forall e v n  y v' t n', (* TODO: A&J counts y here *) *)
-  (*       num_occur_app e v n ->  *)
-  (*       num_occur_app (Eproj v' t n' y e) v (num_occur_list [y] v + n) *)
-  (* | Num_oa_app: *)
-  (*     forall f ys v, *)
-  (*       num_occur_app (Eapp f ys) v (num_occur_list [f] v) *)
-  (* | Num_oa_fun: *)
-  (*     forall e v n m fl, *)
-  (*       num_occur_app e v n -> *)
-  (*       num_occur_app_fds fl v m -> *)
-  (*       num_occur_app (Efun fl e) v (n + m ) *)
-  (* with num_occur_app_fds: fundefs -> var -> nat -> Prop := *)
-  (*      | Num_oa_nil : forall v, *)
-  (*                       num_occur_app_fds Fnil v 0 *)
-  (*      | Num_oa_cons : forall v t n v' ys e fds' m, *)
-  (*                        num_occur_app e v n -> *)
-  (*                        num_occur_app_fds fds' v m -> *)
-  (*                        num_occur_app_fds (Fcons v' t ys e fds') v (n + m). *)
+Definition num_occur_list (lv:list var) (v:var) : nat :=
+  fold_right (fun v' n => if (var_dec v v') then 1 + n
+                          else n) 0 lv.
 
-  (* (* number of times var occurs in exp in an escaping position *) *)
-  (* Inductive num_occur_esc: exp -> var -> nat -> Prop := *)
-  (* | Num_oe_constr: *)
-  (*   forall x t c ys e v n, *)
-  (*     num_occur_esc e v n -> *)
-  (*     num_occur_esc (Econstr x t c ys e) v (n + (num_occur_list ys v)) *)
-  (* | Num_oe_prim: *)
-  (*     forall x t f ys e v n, *)
-  (*       num_occur_esc e v n -> *)
-  (*       num_occur_esc (Eprim x t f ys e) v (n + (num_occur_list ys v)) *)
-  (* | Num_oe_case: *)
-  (*     forall v' cl v, *)
-  (*       num_occur_esc (Ecase v' cl) v (num_occur_list (snd (split cl)) v) *)
-  (* | Num_oe_proj: *)
-  (*     forall e v n  y v' t n', *)
-  (*       num_occur_esc  e v n ->  *)
-  (*       num_occur_esc (Eproj v' t n' y e) v n *)
-  (* | Num_oe_app: *)
-  (*     forall f ys v, *)
-  (*       num_occur_esc (Eapp f ys) v (num_occur_list ys v) *)
-  (* | Num_oe_fun: *)
-  (*     forall e v n m fl, *)
-  (*       num_occur_esc e v n -> *)
-  (*       num_occur_esc_fds fl v m -> *)
-  (*       num_occur_esc (Efun fl e) v (n + m ) *)
-  (* with num_occur_esc_fds: fundefs -> var -> nat -> Prop := *)
-  (*      | Num_oe_nil : *)
-  (*          forall v, *)
-  (*            num_occur_esc_fds Fnil v 0 *)
-  (*      | Num_oe_cons : *)
-  (*          forall v t n v' ys e fds' m, *)
-  (*            num_occur_esc e v n -> *)
-  (*            num_occur_esc_fds fds' v m -> *)
-  (*            num_occur_esc_fds (Fcons v' t ys e fds') v (n + m).   *)
-
-End OCCUR.  
+(* number of time var occurs in exp (free or not) *)
+(* Inductive num_occur: exp -> var -> nat -> Prop := *)
+(* | Num_occ_constr: *)
+(*   forall x t c ys e v n, *)
+(*     num_occur e v n -> *)
+(*     num_occur (Econstr x t c ys e) v (n + (num_occur_list ys v)) *)
+(* | Num_occ_prim: *)
+(*     forall x t f ys e v n, *)
+(*       num_occur e v n -> *)
+(*       num_occur (Eprim x t f ys e) v (n + (num_occur_list ys v)) *)
+(* | Num_occ_case: *)
+(*     forall v' cl v, *)
+(*       num_occur (Ecase v' cl) v (num_occur_list (v'::(snd (split cl))) v) *)
+(* | Num_occ_proj: *)
+(*     forall e v n  y v' t n', *)
+(*       num_occur  e v n ->  *)
+(*       num_occur (Eproj v' t n' y e) v (num_occur_list [y] v + n) *)
+(* | Num_occ_app: *)
+(*     forall f ys v, *)
+(*                  num_occur (Eapp f ys) v (num_occur_list (f::ys) v) *)
+(* | Num_occ_fun: *)
+(*     forall e v n m fl, *)
+(*       num_occur e v n -> *)
+(*       num_occur_fds fl v m -> *)
+(*       num_occur (Efun fl e) v (n + m ) *)
+(* with num_occur_fds: fundefs -> var -> nat -> Prop := *)
+(*      | Num_occ_nil : *)
+(*          forall v, *)
+(*            num_occur_fds Fnil v 0 *)
+(*      | Num_occ_cons : *)
+(*          forall v t n v' ys e fds' m, *)
+(*            num_occur e v n -> *)
+(*            num_occur_fds fds' v m -> *)
+(*            num_occur_fds (Fcons v' t ys e fds') v (n + m). *)
 
 
-Section BINDING.
-
-  Inductive bv_e: exp -> list var -> Prop :=
-  | Constr_bv :
-      forall e l x t c ys, bv_e e l -> bv_e (Econstr x t c ys e) (x::l)
-  | Case_bv :
-      forall v cl, bv_e (Ecase v cl) []
-  | Proj_bv:
-      forall v t n y e l, bv_e e l -> bv_e (Eproj v t n y e) (v::l)
-  | Fun_bv:
-      forall fl e l1 l2, bv_f fl l1 -> bv_e e l2 -> bv_e (Efun fl e) (l1 ++ l2)
-  | App_bv :
-      forall f ys, bv_e (Eapp f ys) []
-  | Prim_bv :
-      forall x t f ys e l, bv_e e l -> bv_e (Eprim x t f ys e) (x::l)
-  with bv_f : fundefs -> list var -> Prop :=
-       | Cons_bv :
-           forall f t ys e fds l1 l2,
-             bv_e e l1 ->
-             bv_f fds l2 ->
-             bv_f (Fcons f t ys e fds) (f::(ys++(l1++l2)))
-       | Nil_bv : bv_f Fnil [].
-
-  Hint Constructors bv_e bv_f.
-  
-  Theorem e_bv_e :
-    forall e, exists l, bv_e e l
-  with e_bv_f: forall f, exists l, bv_f f l.
-  Proof.
-    induction e; destructAll; clear e_bv_e; eauto.
-    specialize (e_bv_f f). destruct e_bv_f. eauto. 
-    induction f; destructAll; clear e_bv_f; eauto.
-    specialize (e_bv_e e); destruct e_bv_e. eauto.
-  Qed.
+(* (* number of times var occurs in a context *) *)
+(* Inductive num_occur_ec: exp_ctx -> var -> nat -> Prop := *)
+(* | Noec_hole: forall v, num_occur_ec Hole_c v 0 *)
+(* | Noec_constr: forall c v n x t ys g, *)
+(*                  num_occur_ec c v n ->  *)
+(*                  num_occur_ec (Econstr_c x t g ys c) v (num_occur_list ys v + n) *)
+(* | Noec_prim: forall c v n x t f ys,  *)
+(*                num_occur_ec c v n ->  *)
+(*                num_occur_ec (Eprim_c x t f ys c) v (num_occur_list ys v + n ) *)
+(* | Noec_proj: forall  v n y v' t n' c, *)
+(*                num_occur_ec c v n -> *)
+(*                num_occur_ec (Eproj_c v' t n' y c) v (num_occur_list [y] v + n) *)
+(* | Noec_fun1: forall n m fds c v, *)
+(*                num_occur_ec c v n -> *)
+(*                num_occur_fds fds v m -> *)
+(*                num_occur_ec (Efun1_c fds c) v (n+m) *)
+(* | Noec_fun2: forall n m fdc e v , *)
+(*                num_occur e v n -> *)
+(*                num_occur_fdc fdc v m -> *)
+(*                num_occur_ec (Efun2_c fdc e) v (n + m) *)
+(* with num_occur_fdc : fundefs_ctx -> var -> nat -> Prop := *)
+(*      | Nofc_fcons1 : forall v n m fds t ys c f, *)
+(*                        num_occur_ec c v n -> *)
+(*                        num_occur_fds fds v m ->  *)
+(*                        num_occur_fdc (Fcons1_c f t ys c fds) v  (n + m) *)
+(*      | Nofc_fcons2 : forall e v n m fdc f t ys, *)
+(*                        num_occur e v n -> *)
+(*                        num_occur_fdc fdc v m -> *)
+(*                        num_occur_fdc (Fcons2_c f t ys e fdc) v (n + m). *)
 
 
-  
+(* (* number of times var occurs in exp in an applied position *) *)
+(* Inductive num_occur_app: exp -> var -> nat -> Prop := *)
+(* | Num_oa_constr: *)
+(*   forall x t c ys e v n, *)
+(*     num_occur_app e v n -> num_occur_app (Econstr x t c ys e) v n *)
+(* | Num_oa_prim: *)
+(*     forall x t f ys e v n, *)
+(*       num_occur_app e v n -> num_occur_app (Eprim x t f ys e) v n *)
+(* | Num_oa_case: *)
+(*     forall v' cl v, *)
+(*       num_occur_app (Ecase v' cl) v (num_occur_list [v'] v) *)
+(* | Num_oa_proj: *)
+(*     forall e v n  y v' t n', (* TODO: A&J counts y here *) *)
+(*       num_occur_app e v n ->  *)
+(*       num_occur_app (Eproj v' t n' y e) v (num_occur_list [y] v + n) *)
+(* | Num_oa_app: *)
+(*     forall f ys v, *)
+(*       num_occur_app (Eapp f ys) v (num_occur_list [f] v) *)
+(* | Num_oa_fun: *)
+(*     forall e v n m fl, *)
+(*       num_occur_app e v n -> *)
+(*       num_occur_app_fds fl v m -> *)
+(*       num_occur_app (Efun fl e) v (n + m ) *)
+(* with num_occur_app_fds: fundefs -> var -> nat -> Prop := *)
+(*      | Num_oa_nil : forall v, *)
+(*                       num_occur_app_fds Fnil v 0 *)
+(*      | Num_oa_cons : forall v t n v' ys e fds' m, *)
+(*                        num_occur_app e v n -> *)
+(*                        num_occur_app_fds fds' v m -> *)
+(*                        num_occur_app_fds (Fcons v' t ys e fds') v (n + m). *)
+
+(* (* number of times var occurs in exp in an escaping position *) *)
+(* Inductive num_occur_esc: exp -> var -> nat -> Prop := *)
+(* | Num_oe_constr: *)
+(*   forall x t c ys e v n, *)
+(*     num_occur_esc e v n -> *)
+(*     num_occur_esc (Econstr x t c ys e) v (n + (num_occur_list ys v)) *)
+(* | Num_oe_prim: *)
+(*     forall x t f ys e v n, *)
+(*       num_occur_esc e v n -> *)
+(*       num_occur_esc (Eprim x t f ys e) v (n + (num_occur_list ys v)) *)
+(* | Num_oe_case: *)
+(*     forall v' cl v, *)
+(*       num_occur_esc (Ecase v' cl) v (num_occur_list (snd (split cl)) v) *)
+(* | Num_oe_proj: *)
+(*     forall e v n  y v' t n', *)
+(*       num_occur_esc  e v n ->  *)
+(*       num_occur_esc (Eproj v' t n' y e) v n *)
+(* | Num_oe_app: *)
+(*     forall f ys v, *)
+(*       num_occur_esc (Eapp f ys) v (num_occur_list ys v) *)
+(* | Num_oe_fun: *)
+(*     forall e v n m fl, *)
+(*       num_occur_esc e v n -> *)
+(*       num_occur_esc_fds fl v m -> *)
+(*       num_occur_esc (Efun fl e) v (n + m ) *)
+(* with num_occur_esc_fds: fundefs -> var -> nat -> Prop := *)
+(*      | Num_oe_nil : *)
+(*          forall v, *)
+(*            num_occur_esc_fds Fnil v 0 *)
+(*      | Num_oe_cons : *)
+(*          forall v t n v' ys e fds' m, *)
+(*            num_occur_esc e v n -> *)
+(*            num_occur_esc_fds fds' v m -> *)
+(*            num_occur_esc_fds (Fcons v' t ys e fds') v (n + m).   *)
+
+Inductive bv_e: exp -> list var -> Prop :=
+| Constr_bv :
+    forall e l x t c ys, bv_e e l -> bv_e (Econstr x t c ys e) (x::l)
+| Case_bv :
+    forall v cl, bv_e (Ecase v cl) []
+| Proj_bv:
+    forall v t n y e l, bv_e e l -> bv_e (Eproj v t n y e) (v::l)
+| Fun_bv:
+    forall fl e l1 l2, bv_f fl l1 -> bv_e e l2 -> bv_e (Efun fl e) (l1 ++ l2)
+| App_bv :
+    forall f ys, bv_e (Eapp f ys) []
+| Prim_bv :
+    forall x t f ys e l, bv_e e l -> bv_e (Eprim x t f ys e) (x::l)
+with bv_f : fundefs -> list var -> Prop :=
+     | Cons_bv :
+         forall f t ys e fds l1 l2,
+           bv_e e l1 ->
+           bv_f fds l2 ->
+           bv_f (Fcons f t ys e fds) (f::(ys++(l1++l2)))
+     | Nil_bv : bv_f Fnil [].
+
+Hint Constructors bv_e bv_f.
+
+Theorem e_bv_e :
+  forall e, exists l, bv_e e l
+                      with e_bv_f: forall f, exists l, bv_f f l.
+Proof.
+  induction e; destructAll; clear e_bv_e; eauto.
+  specialize (e_bv_f f). destruct e_bv_f. eauto. 
+  induction f; destructAll; clear e_bv_f; eauto.
+  specialize (e_bv_e e); destruct e_bv_e. eauto.
+Qed.
+
+
+
 (*   
   Theorem bv_e_det: forall e l1 l2, bv_e e l1 -> bv_e e l2 -> l1 = l2
    with bv_f_det: forall f l1 l2, bv_f f l1 -> bv_f f l2 -> l1 = l2.                     
@@ -285,22 +273,34 @@ Section BINDING.
       + reflexivity.
   Qed.
  *)
-  
 
-  
-End BINDING.
+Theorem findtag_not_empty:
+  forall A cl (k:A) (v:tag), findtag cl v = Some k -> 0 < (length cl).
+Proof.
+  induction cl; intros.
+  - inversion H.
+  - simpl in H. destruct a. destruct (M.elt_eq t v).
+    + inversion H. simpl. omega.
+    + simpl. apply IHcl in H. omega.
+Qed.
 
-Section OTHER.
+Inductive split_fds: fundefs -> fundefs -> fundefs -> Prop :=
+| Left_f:
+    forall lfds rfds lrfds v t ys e,
+      split_fds lfds rfds lrfds ->
+      split_fds (Fcons v t ys e lfds) rfds (Fcons v t ys e lrfds)
+| Right_f:
+    forall lfds rfds lrfds v t ys e,
+      split_fds lfds rfds lrfds ->
+      split_fds lfds (Fcons v t ys e rfds) (Fcons v t ys e lrfds)
+| End_f: split_fds Fnil Fnil Fnil.
 
-  Theorem findtag_not_empty:
-    forall A cl (k:A) (v:tag), findtag cl v = Some k -> 0 < (length cl).
-  Proof.
-    induction cl; intros.
-    - inversion H.
-    - simpl in H. destruct a. destruct (M.elt_eq t v).
-      + inversion H. simpl. omega.
-      + simpl. apply IHcl in H. omega.
-  Qed.
+(** easy lemmas about split_fds. 
+    TODO move split_fds in common file along with lemmas *)
+Lemma split_fds_nil_l fdefs : split_fds fdefs Fnil fdefs.
+  induction fdefs; constructor; eauto.
+Qed.
 
-  
-End OTHER.  
+Lemma split_fds_nil_r fdefs : split_fds Fnil fdefs fdefs.
+  induction fdefs; constructor; eauto.
+Qed.
